make closure_interp/type_interp opaque

theories/iris/logrel.v
@@ -1046,11 +1046,28 @@ Section instr.
     | CodeRefT _ ϕ => coderef_interp (closure_interp ϕ)
     end%I.
 
+  Definition closure_interp' (ϕ : function_type) : semantic_env -n> ClR :=
+    match ϕ with
+    | MonoFunT τs1 τs2 => mono_closure_interp τs1 τs2 (map type_interp τs1) (map type_interp τs2)
+    | ForallMemT ϕ' => forall_mem_interp (closure_interp ϕ')
+    | ForallRepT ϕ' => forall_rep_interp (closure_interp ϕ')
+    | ForallSizeT ϕ' => forall_size_interp (closure_interp ϕ')
+    | ForallTypeT κ ϕ' => forall_type_interp κ (closure_interp ϕ')
+    end%I.
+
   Lemma type_interp_eq τ se sv :
     type_interp τ se sv ⊣⊢ (add_skind_interp τ $ pre_type_interp τ) se sv.
   Proof.
     destruct τ; reflexivity.
   Qed.
+
+  Lemma closure_interp_eq ϕ se cl :
+    closure_interp ϕ se cl ⊣⊢ closure_interp' ϕ se cl.
+  Proof.
+    by destruct ϕ.
+  Qed.
+
+  Opaque type_interp closure_interp.
 
   Program Definition value_interp : semantic_env -n> leibnizO type -n> SVR := λne se τ, type_interp τ se.
   Next Obligation. solve_proper. Qed.
